Preservation prove
* Add jdgBinOp jdgLetIn in TypeJdg

* Change to Hash map

LocalLang/Typing.lean
@@ -5,13 +5,21 @@ import LocalLang.Types
 
 mutual
   inductive TypeJdg : TypeContext → Expr → LLType → Prop where
-    | jdgVar {Γ : TypeContext}  {name : String} (H : (name, LLType.nat) ∈ Γ)
-                      : TypeJdg Γ (.var name) LLType.nat
-    | jdgConst {Γ : TypeContext} {n : ℕ} : TypeJdg Γ (.const n) LLType.nat
-    | jdgFun {Γ : TypeContext} {es : List Expr} {arg_types : List LLType} {T_return : LLType}
-                  (H_f : (f, .func arg_types T_return) ∈ Γ)
+    | jdg_var {Γ : TypeContext}  {name : String} {ty : LLType} (H : Γ[name]? = some ty)
+                      : TypeJdg Γ (.var name) ty
+    | jdg_const {Γ : TypeContext} {n : ℕ} : TypeJdg Γ (.const n) LLType.nat
+    | jdg_fun {f} {Γ : TypeContext} {es : List Expr} {arg_types : List LLType} {T_return : LLType}
+                  (H_f : Γ[f]? = some (.func arg_types T_return))
                   (H_args : TypeJdgList Γ es arg_types)
                         : TypeJdg Γ (.funCall f es) (LLType.func arg_types T_return)
+    | jdg_binOp {Γ : TypeContext} {op : BinOp} {e₁ e₂ : Expr}
+                (H₁ : TypeJdg Γ e₁ LLType.nat) (H₂ : TypeJdg Γ e₂ LLType.nat)
+                        : TypeJdg Γ (.binOp op e₁ e₂) .nat
+    | jdg_let_in {Γ : TypeContext} {name : String} {e₁ e₂ : Expr} {ty₁ ty₂ : LLType}
+                (H₁ : TypeJdg Γ e₁ ty₁)
+                (H₂ : TypeJdg (Γ.insert name ty₁) e₂ ty₂)
+                        : TypeJdg  Γ (.letIn name e₁ e₂) ty₂
+
 
   inductive TypeJdgList : TypeContext -> List Expr -> List LLType -> Prop
     | nil : TypeJdgList Γ [] []
