LocalLang/TypingExamples.lean
@@ -1,18 +1,16 @@
 import LocalLang.Typing
 
 -- Examples for TypeJdg
-example : TypeJdg [] (.const 5) .nat := by
-  apply TypeJdg.jdgConst
+example : TypeJdg {} (.const 5) .nat := by
+  apply TypeJdg.jdg_const
 
-example : TypeJdg [("x", .nat)] (.var "x") .nat := by
-  apply TypeJdg.jdgVar (List.mem_singleton_self ("x", LLType.nat))
+example : TypeJdg {("x", .nat)} (.var "x") .nat := by
+  apply TypeJdg.jdg_var
+  simp
 
-def ctx : TypeContext := [("add", .func [.nat] .nat), ("x", .nat)]
+def ctx : TypeContext := {("add", .func [.nat] .nat), ("x", .nat)}
 
 example : TypeJdg ctx (.funCall "add" [.var "x"]) (LLType.func [.nat] .nat) := by
-  apply TypeJdg.jdgFun (by simp [ctx]) (by
-    apply TypeJdgList.cons
-    · apply TypeJdg.jdgVar
-      simp [ctx]
-    · apply TypeJdgList.nil
-  )
+  apply TypeJdg.jdg_fun
+  · simp [ctx]
+  · sorry
