LocalLang/TypingGuarantees.lean
@@ -3,10 +3,35 @@ import LocalLang.Semantics
 import LocalLang.Types
 import LocalLang.Typing
 
+def EnvRespectsCtx (Γ : TypeContext) (V : Env) : Prop :=
+  ∀ (x : String) (n : ℕ), V[x]? = some n → Γ[x]? = LLType.nat
+
 -- TODO: prove
 -- TODO: V and Γ should be related
 theorem preservation (Γ : TypeContext) (e e' : Expr) (ty : LLType) (defs : Definitions)
-  : TypeJdg Γ e ty → SmallStep defs V e e' → TypeJdg Γ e' ty := sorry
+    (h_env_respects : EnvRespectsCtx Γ V)
+  : TypeJdg Γ e ty → HeadSmallStep defs V e e' → TypeJdg Γ e' ty := by
+  intro h_jdg b
+  induction b
+  · cases h_jdg
+    · rename_i x n a relΓ
+      unfold EnvRespectsCtx at h_env_respects
+      let ent_ctx_link := h_env_respects x n a
+      let symmRelΓ := relΓ.symm
+      have ty_eq := Option.some.inj (symmRelΓ.trans ent_ctx_link)
+      rw [ty_eq]
+      constructor
+  · cases h_jdg
+    · rename_i H₁ H₂
+      apply TypeJdg.jdg_const
+  · rename_i name val n
+    cases h_jdg
+    · rename_i H₁ H₂
+      cases H₂
+      constructor
+  · cases h_jdg
+    rename_i f es arg_types T_return h_f h_args
+    sorry
 
 -- Progress: if TypeJdg Γ e ty, then e can take a step.
 -- TODO: formalize
